examples/BoundedQueueCode.v
@@ -1,0 +1,279 @@
+From Coq Require Import List.
+From examples Require Import CAL.
+From compcert Require Import
+     Integers Coqlib Maps
+     Memory AST Values
+     Clight Ctypes
+     LanguageInterface
+     Events Globalenvs
+     Smallstep.
+Import ListNotations.
+
+(** identifies for the functions *)
+Definition set_id: positive := 101.
+Definition get_id: positive := 102.
+Definition inc1_id: positive := 103.
+Definition inc2_id: positive := 104.
+Definition enq_id: positive := 105.
+Definition deq_id: positive := 106.
+(** identifiers for the global variables *)
+Definition arr_id: positive := 1.
+Definition cnt1_id: positive := 2.
+Definition cnt2_id: positive := 3.
+(** identifiers for the arguments  *)
+Definition get_arg_id: positive := 1.
+Definition set_arg1_id: positive := 1.
+Definition set_arg2_id: positive := 2.
+Definition enq_arg_id: positive := 1.
+(** identifiers for the temps *)
+Definition rb_inc1_tmp : positive := 1.
+Definition rb_inc2_tmp : positive := 1.
+Definition bq_enq_tmp : positive := 2.
+Definition bq_deq_tmp1 : positive := 1.
+Definition bq_deq_tmp2 : positive := 2.
+
+Notation tint := (Tint I32 Unsigned noattr).
+Notation tarray := (fun ty size => Tarray ty size noattr).
+Notation tptr := (fun ty => Tpointer ty noattr).
+Notation tvoid := (Tvoid).
+
+Definition Nz: Z := Z.of_nat CAL.N.
+
+Section CLIGHT.
+
+  Definition inc1_sg: signature :=
+    signature_of_type Tnil tint cc_default.
+  Definition inc2_sg: signature :=
+    signature_of_type Tnil tint cc_default.
+  Definition get_sg: signature :=
+    signature_of_type (Tcons tint Tnil) tint cc_default.
+  Definition set_sg: signature :=
+    signature_of_type (Tcons tint (Tcons tint Tnil)) tvoid cc_default.
+  Definition enq_sg: signature :=
+    signature_of_type (Tcons tint Tnil) tvoid cc_default.
+  Definition deq_sg: signature :=
+    signature_of_type Tnil tint cc_default.
+
+  (**
+<<
+    int get(int i) {
+      return arr[i];
+    }
+>>
+   *)
+  Definition rb_get_body : statement :=
+    Sreturn
+      (Some
+         (Ederef
+            (Ebinop Cop.Oadd
+                    (Evar arr_id (tarray tint Nz))
+                    (Etempvar get_arg_id tint)
+                    (tptr tint))
+            tint)).
+  Definition rb_get : function :=
+    {|
+      fn_return := tint;
+      fn_callconv := cc_default;
+      fn_params := [(get_arg_id, tint)];
+      fn_vars := [];
+      fn_temps := [];
+      fn_body := rb_get_body;
+    |}.
+
+  (**
+<<
+    void set(int i, int v) {
+      arr[i] = v;
+    }
+>>
+   *)
+  Definition rb_set_body : statement :=
+    Ssequence
+      (Sassign
+         (Ederef
+            (Ebinop Cop.Oadd
+                    (Evar arr_id (tarray tint Nz))
+                    (Etempvar set_arg1_id tint)
+                    (tptr tint))
+            tint)
+         (Etempvar set_arg2_id tint))
+      (Sreturn None).
+  Definition rb_set : function :=
+    {|
+      fn_return := tvoid;
+      fn_callconv := cc_default;
+      fn_params := [(set_arg1_id, tint); (set_arg2_id, tint)];
+      fn_vars := [];
+      fn_temps := [];
+      fn_body := rb_set_body;
+    |}.
+  (**
+<<
+    int inc1() {
+      int i = cnt1;
+      cnt1 += 1;
+      cnt1 %= N;
+      return i;
+    }
+>>
+   *)
+  Definition rb_inc1_body : statement :=
+    Ssequence
+      (Ssequence
+         (Ssequence
+            (Sset rb_inc1_tmp (Evar cnt1_id tint))
+            (Sassign
+               (Evar cnt1_id tint)
+               (Ebinop Cop.Oadd
+                       (Evar cnt1_id tint)
+                       (Econst_int (Int.repr 1) tint)
+                       tint)))
+         (Sassign
+            (Evar cnt1_id tint)
+            (Ebinop Cop.Omod
+                    (Evar cnt1_id tint)
+                    (Econst_int (Int.repr Nz) tint)
+                    tint)))
+      (Sreturn (Some (Etempvar rb_inc1_tmp tint))).
+  Definition rb_inc1 : function :=
+    {|
+      fn_return := tint;
+      fn_callconv := cc_default;
+      fn_params := [];
+      fn_vars := [];
+      fn_temps := [ (rb_inc1_tmp, tint) ];
+      fn_body := rb_inc1_body;
+    |}.
+
+  (**
+<<
+    int inc2() {
+      int i = cnt1;
+      cnt1 += 1;
+      cnt1 %= N;
+      return i;
+    }
+>>
+  *)
+  Definition rb_inc2_body : statement :=
+    Ssequence
+      (Ssequence
+         (Ssequence
+            (Sset rb_inc2_tmp (Evar cnt2_id tint))
+            (Sassign
+               (Evar cnt2_id tint)
+               (Ebinop Cop.Oadd
+                       (Evar cnt2_id tint)
+                       (Econst_int (Int.repr 1) tint)
+                       tint)))
+         (Sassign
+            (Evar cnt2_id tint)
+            (Ebinop Cop.Omod
+                    (Evar cnt2_id tint)
+                    (Econst_int (Int.repr Nz) tint)
+                    tint)))
+      (Sreturn (Some (Etempvar rb_inc2_tmp tint))).
+  Definition rb_inc2 : function :=
+    {|
+      fn_return := tvoid;
+      fn_callconv := cc_default;
+      fn_params := [];
+      fn_vars := [];
+      fn_temps := [];
+      fn_body := rb_inc2_body;
+    |}.
+  (* FIXME: *)
+  Definition arr_gvar : globvar type :=
+    {|
+      gvar_info := tarray tint Nz;
+      gvar_init := [Init_space (Nz * 4)];
+      gvar_readonly := false;
+      gvar_volatile := false;
+    |}.
+  Program Definition rb_program: Clight.program :=
+    {|
+      prog_defs := [(get_id, Gfun (Internal rb_get));
+        (set_id, Gfun (Internal rb_set));
+        (inc1_id, Gfun (Internal rb_inc1));
+        (inc2_id, Gfun (Internal rb_inc2));
+        (arr_id, Gvar arr_gvar)];
+      prog_public := [get_id; set_id; inc1_id; inc2_id];
+      prog_main := 999%positive;
+      prog_types := [];
+      prog_comp_env := (PTree.empty _);
+    |}.
+
+  (**
+<<
+    void enq(int v) {
+      int i = inc2();
+      set(i, v);
+    }
+>>
+   *)
+  Definition bq_enq_body : statement :=
+    Ssequence
+      (Scall (Some bq_enq_tmp) (Evar inc2_id (Tfunction Tnil tint cc_default)) nil)
+      (Ssequence
+         (Scall None (Evar set_id (Tfunction (Tcons tint (Tcons tint Tnil)) tvoid cc_default))
+                ([Etempvar bq_enq_tmp tint; Etempvar enq_arg_id tint]))
+         (Sreturn None)).
+  Definition bq_enq : function :=
+    {|
+      fn_return := tvoid;
+      fn_callconv := cc_default;
+      fn_params := [(enq_arg_id, tint)];
+      fn_vars := [];
+      fn_temps := [(bq_enq_tmp, tint)];
+      fn_body := bq_enq_body;
+    |}.
+
+  (**
+<<
+    int deq() {
+      int i = inc1();
+      return get(i);
+    }
+>>
+   *)
+  Definition bq_deq_body : statement :=
+    Ssequence
+      (Scall (Some bq_deq_tmp1) (Evar inc1_id (Tfunction Tnil tint cc_default)) nil)
+      (Ssequence
+         (Scall (Some bq_deq_tmp2) (Evar get_id (Tfunction (Tcons tint Tnil) tint cc_default))
+                ([Evar bq_deq_tmp1 tint]))
+         (Sreturn (Some (Evar bq_deq_tmp2 tint)))).
+  Definition bq_deq : function :=
+    {|
+      fn_return := tint;
+      fn_callconv := cc_default;
+      fn_params := [];
+      fn_vars := [];
+      fn_temps := [(bq_deq_tmp1, tint); (bq_deq_tmp2, tint)];
+      fn_body := bq_enq_body;
+    |}.
+
+  Definition inc1_ext: fundef function :=
+    External (EF_external "inc1" inc1_sg) Tnil tint cc_default.
+  Definition inc2_ext: fundef function :=
+    External (EF_external "inc2" inc2_sg) Tnil tint cc_default.
+  Definition get_ext: fundef function :=
+    External (EF_external "get" get_sg) (Tcons tint Tnil) tint cc_default.
+  Definition set_ext: fundef function :=
+    External (EF_external "set" set_sg) (Tcons tint (Tcons tint Tnil)) tvoid cc_default.
+
+  Program Definition bq_program : Clight.program :=
+    {|
+      prog_defs := [(enq_id, Gfun (Internal bq_enq));
+                    (deq_id, Gfun (Internal bq_deq));
+                    (inc1_id, Gfun inc1_ext);
+                    (inc2_id, Gfun inc2_ext);
+                    (get_id, Gfun get_ext);
+                    (set_id, Gfun set_ext)];
+      prog_public := [enq_id; deq_id];
+      prog_main := 999%positive;
+      prog_types := [];
+      prog_comp_env := (PTree.empty _);
+    |}.
+
+End CLIGHT.
